renaming and refactoring

ironfleet/src/Dafny/Distributed/Protocol/RSL/FailureProof/Phase2Proof.i.dfy
@@ -18,20 +18,20 @@ import opened CommonProof__Constants_i
 *****************************************************************************************/
 
 /* Main performance guarantee for phase 2 post-failure */
-predicate PerformanceGuarantee(s:TimestampedRslState, opn:OperationNumber){
-    && PerformanceGuarantee_Response(s)
-    && PerformanceGuarantee_2b(s)
-    && PerformanceGuarantee_2a(s, opn)
+predicate PerformanceGuarantee(ts:TimestampedRslState, opn:OperationNumber){
+    && PerformanceGuarantee_Response(ts)
+    && PerformanceGuarantee_2b(ts)
+    && PerformanceGuarantee_2a(ts, opn)
 }
 
-predicate PerformanceGuarantee_Response(s:TimestampedRslState) {
-    // 0 < |s.constants.config.replica_ids|
+predicate PerformanceGuarantee_Response(ts:TimestampedRslState) {
+    // 0 < |ts.constants.config.replica_ids|
     //     && (forall pkt :: 
-    //             && pkt in s.undeliveredPackets
+    //             && pkt in ts.undeliveredPackets
     //             && pkt.msg.v.RslMessage_Reply?
-    //             && pkt.src == s.constants.config.replica_ids[0]
+    //             && pkt.src == ts.constants.config.replica_ids[0]
     //             ==>
-    //             TimeLe(pkt.msg.ts, TimeBoundReply(req_time, s.constants))
+    //             TimeLe(pkt.msg.ts, TimeBoundReply(req_time, ts.constants))
     //     )
     //TODO
     true
@@ -42,9 +42,9 @@ predicate PerformanceGuarantee_2b(b:TimestampedRslState) {
     true
 }
 
-predicate PerformanceGuarantee_2a(s:TimestampedRslState, opn:OperationNumber) {
+predicate PerformanceGuarantee_2a(ts:TimestampedRslState, opn:OperationNumber) {
     forall pkt {:trigger pkt.msg.v.RslMessage_2a?} | 
-        && pkt in s.undeliveredPackets 
+        && pkt in ts.undeliveredPackets 
         && IsNew2aPacket(pkt, opn)
     :: TimeLe(pkt.msg.ts, TimeBound2aDeliveryPost())
 }
@@ -58,69 +58,69 @@ function TimeBound2aDeliveryPost() : Timestamp {
 *****************************************************************************************/
 
 /* Conjunction of all assumptions */
-predicate RslAssumption(s:TimestampedRslState)
+predicate RslAssumption(ts:TimestampedRslState)
 {
     && RelationsAssumptions()
-    && RslConsistency(s)
-    && NoPacketDuplication(s)
-    && |s.t_replicas| > 2  // For failure to be meaningful
-    && s.constants.params.max_batch_size == 1
+    && RslConsistency(ts)
+    && NoPacketDuplication(ts)
+    && |ts.t_replicas| > 2  // For failure to be meaningful
+    && ts.constants.params.max_batch_size == 1
 
-    && (var nextStep := s.t_environment.nextStep; 
+    && (var nextStep := ts.t_environment.nextStep; 
     nextStep.LEnvStepHostIos? ==>
     (forall io | io in nextStep.ios && io.LIoOpReceive? :: !io.r.msg.v.RslMessage_Heartbeat? && !io.r.msg.v.RslMessage_Request?))
-    && LeaderAlwaysOne(s)
+    && LeaderAlwaysOne(ts)
     && minD < SelfDelivery < D < 2*minD
     && ProcessPacket > 0
     && SelfDelivery + TimeActionRange(0) < D
-    && NoExternalPackets(s)
-    && NoExternalSteps(s)
-    && BoundedQueueingAssumption(s)
+    && NoExternalPackets(ts)
+    && NoExternalSteps(ts)
+    && BoundedQueueingAssumption(ts)
 }
 
 predicate RelationsAssumptions() {
     && TimeLe(req_time, NewLeaderInitTS)
 }
 
-predicate LeaderAlwaysOne(s:TimestampedRslState) 
-    requires |s.t_replicas| > 2
+predicate LeaderAlwaysOne(ts:TimestampedRslState) 
+    requires |ts.t_replicas| > 2
 {
-    && (forall idx | 0 <= idx < |s.t_replicas| && idx != 1
-        :: s.t_replicas[idx].v.replica.proposer.current_state == 0)
-    && s.t_replicas[1].v.replica.proposer.current_state == 2
-    && s.t_replicas[1].v.replica.proposer.election_state.current_view == Ballot(1, 1)
+    && (forall idx | 0 <= idx < |ts.t_replicas| && idx != 1
+        :: ts.t_replicas[idx].v.replica.proposer.current_state == 0)
+    && ts.t_replicas[1].v.replica.proposer.current_state == 2
+    && ts.t_replicas[1].v.replica.proposer.election_state.current_view == Ballot(1, 1)
 }
 
-predicate NoExternalPackets(s:TimestampedRslState) {
-    forall pkt | pkt in s.undeliveredPackets ::
-        && pkt in s.t_environment.sentPackets
-        && pkt.src in s.constants.config.replica_ids
-        && pkt.dst in s.constants.config.replica_ids
+predicate NoExternalPackets(ts:TimestampedRslState) {
+    forall pkt | pkt in ts.undeliveredPackets ::
+        && pkt in ts.t_environment.sentPackets
+        && pkt.src in ts.constants.config.replica_ids
+        && pkt.dst in ts.constants.config.replica_ids
 }
 
-predicate NoExternalSteps(s:TimestampedRslState) {
-    !(exists eid, ios :: s.t_environment.nextStep == LEnvStepHostIos(eid, ios, ExternalStep()))
+predicate NoExternalSteps(ts:TimestampedRslState) {
+    !(exists eid, ios :: ts.t_environment.nextStep == LEnvStepHostIos(eid, ios, ExternalStep()))
 }
 
 // Bounded queueing assumption for simplified RSL
-predicate BoundedQueueingAssumption(s:TimestampedRslState) 
-    requires RslConsistency(s)
+predicate BoundedQueueingAssumption(ts:TimestampedRslState) 
+    requires RslConsistency(ts)
 {
     forall idx, ios :: (
-        && 0 <= idx < |s.constants.config.replica_ids|
-        && s.t_environment.nextStep == LEnvStepHostIos(s.constants.config.replica_ids[idx], ios, RslStep(s.t_replicas[idx].v.nextActionIndex))
+        && 0 <= idx < |ts.constants.config.replica_ids|
+        && ts.t_environment.nextStep == LEnvStepHostIos(ts.constants.config.replica_ids[idx], ios, RslStep(ts.t_replicas[idx].v.nextActionIndex))
         ==>
-        (forall io | io in s.t_environment.nextStep.ios && io.LIoOpReceive? ::
+        (forall io | io in ts.t_environment.nextStep.ios && io.LIoOpReceive? ::
             // this means that max(replica.ts, msg.ts) <= msg.ts + MaxQueueTime
-            s.t_replicas[idx].ts <= io.r.msg.ts + MaxQueueTime
+            ts.t_replicas[idx].ts <= io.r.msg.ts + MaxQueueTime
         )
     )
 }
 
-predicate RslConsistency(s:TimestampedRslState)
+predicate RslConsistency(ts:TimestampedRslState)
 {
-    ConstantsAllConsistentInv(UntimestampRslState(s))
-        && WellFormedLConfiguration(s.constants.config)
+    ConstantsAllConsistentInv(UntimestampRslState(ts))
+        && WellFormedLConfiguration(ts.constants.config)
 }
 
 
@@ -134,39 +134,39 @@ ghost const req_time:Timestamp
 ghost const NewLeaderInitTS:Timestamp
 
 //  Invariant of starting state of Phase2 proof
-predicate BoundaryCond(s:TimestampedRslState, opn:OperationNumber) 
-    requires |s.t_replicas| > 2
+predicate BoundaryCond(ts:TimestampedRslState, opn:OperationNumber) 
+    requires |ts.t_replicas| > 2
 {
-    && BoundaryCond_ExistingPacketsBallot(s)
-    && BoundaryCond_NewLeader(s, opn)
+    && BoundaryCond_ExistingPacketsBallot(ts)
+    && BoundaryCond_NewLeader(ts, opn)
 }
 
 
-predicate BoundaryCond_NewLeader(s:TimestampedRslState, opn:OperationNumber) 
-    requires |s.t_replicas| > 2
+predicate BoundaryCond_NewLeader(ts:TimestampedRslState, opn:OperationNumber) 
+    requires |ts.t_replicas| > 2
 {
-    var r := s.t_replicas[1].v.replica;
-    && s.t_replicas[1].v.nextActionIndex == 3
+    var r := ts.t_replicas[1].v.replica;
+    && ts.t_replicas[1].v.nextActionIndex == 3
     && r.proposer.current_state == 2
     && r.proposer.election_state.current_view == Ballot(1, 1)
     && r.proposer.max_ballot_i_sent_1a == Ballot(1, 1)
     && opn == r.proposer.next_operation_number_to_propose
     && opn == r.executor.ops_complete
-    && LeaderSet1bContainsRequest(s)
-    && s.t_replicas[1].v.replica.proposer.request_queue == []
+    && LeaderSet1bContainsRequest(ts)
+    && ts.t_replicas[1].v.replica.proposer.request_queue == []
 }
 
-predicate LeaderSet1bContainsRequest(s:TimestampedRslState) 
-    requires |s.t_replicas| > 2
+predicate LeaderSet1bContainsRequest(ts:TimestampedRslState) 
+    requires |ts.t_replicas| > 2
 {
-    var r := s.t_replicas[1].v.replica;
+    var r := ts.t_replicas[1].v.replica;
     && LProposerCanNominateUsingOperationNumber(r.proposer, r.acceptor.log_truncation_point, r.proposer.next_operation_number_to_propose)
     && !LAllAcceptorsHadNoProposal(r.proposer.received_1b_packets, r.proposer.next_operation_number_to_propose)
 }
 
 
-predicate BoundaryCond_ExistingPacketsBallot(s:TimestampedRslState) {
-    forall pkt | pkt in s.undeliveredPackets :: Boundary_ExistingPacketsBallot(pkt)
+predicate BoundaryCond_ExistingPacketsBallot(ts:TimestampedRslState) {
+    forall pkt | pkt in ts.undeliveredPackets :: Boundary_ExistingPacketsBallot(pkt)
 }
 predicate Boundary_ExistingPacketsBallot(pkt:TimestampedLPacket<EndPoint, RslMessage>) {
     match pkt.msg.v {
@@ -200,55 +200,56 @@ predicate Boundary_ExistingPacketsBallot(pkt:TimestampedLPacket<EndPoint, RslMes
 
 
 // Main invariant 
-predicate RslPerfInvariant(s:TimestampedRslState, opn:OperationNumber) 
-    requires |s.t_replicas| > 2
+predicate RslPerfInvariant(ts:TimestampedRslState, opn:OperationNumber) 
+    requires |ts.t_replicas| > 2
 {
-    && RslConsistency(s)
-    && AlwaysInvariant(s)
-    && PerformanceGuarantee(s, opn)
-    && PacketsBallotInvariant(s)
-    && (|| Before_2a_Sent_Invariant(s, opn)
-        || After_2a_Sent_Invariant(s, opn)
+    && RslConsistency(ts)
+    && AlwaysInvariant(ts)
+    && PerformanceGuarantee(ts, opn)
+    && PacketsBallotInvariant(ts)
+    && (|| Before_2a_Sent_Invariant(ts, opn)
+        || Before_2b_Sent_Invariant(ts, opn)
+        || After_2b_Sent_Invariant(ts, opn)
     )
 }
 
 
-predicate ServersAreNotClients(s:TimestampedRslState)
+predicate ServersAreNotClients(ts:TimestampedRslState)
 {
-  forall id :: id in s.constants.config.clientIds && id in s.constants.config.replica_ids
+  forall id :: id in ts.constants.config.clientIds && id in ts.constants.config.replica_ids
     ==> false
 }
 
-predicate RequestBatchSrcInClientIds(s:TimestampedRslState, v:RequestBatch)
+predicate RequestBatchSrcInClientIds(ts:TimestampedRslState, v:RequestBatch)
 {
-  forall r :: r in v ==> r.client in s.constants.config.clientIds
+  forall r :: r in v ==> r.client in ts.constants.config.clientIds
 }
 
-predicate AlwaysInvariant(s:TimestampedRslState)
-    requires |s.t_replicas| > 2
+predicate AlwaysInvariant(ts:TimestampedRslState)
+    requires |ts.t_replicas| > 2
 {
-    && ServersAreNotClients(s)
-    && s.t_replicas[1].v.replica.proposer.request_queue == []
-    && (forall pkt | pkt in s.undeliveredPackets :: pkt in s.t_environment.sentPackets)
-    && (forall pkt | pkt in s.undeliveredPackets && pkt.msg.v.RslMessage_2a? :: RequestBatchSrcInClientIds(s, pkt.msg.v.val_2a))
-    && (forall pkt | pkt in s.undeliveredPackets && pkt.msg.v.RslMessage_2b? :: RequestBatchSrcInClientIds(s, pkt.msg.v.val_2b))
-    && (forall pkt | pkt in s.t_replicas[1].v.replica.proposer.received_1b_packets && pkt.msg.RslMessage_1b? :: forall op | op in pkt.msg.votes :: RequestBatchSrcInClientIds(s, pkt.msg.votes[op].max_val))
+    && ServersAreNotClients(ts)
+    && ts.t_replicas[1].v.replica.proposer.request_queue == []
+    && (forall pkt | pkt in ts.undeliveredPackets :: pkt in ts.t_environment.sentPackets)
+    && (forall pkt | pkt in ts.undeliveredPackets && pkt.msg.v.RslMessage_2a? :: RequestBatchSrcInClientIds(ts, pkt.msg.v.val_2a))
+    && (forall pkt | pkt in ts.undeliveredPackets && pkt.msg.v.RslMessage_2b? :: RequestBatchSrcInClientIds(ts, pkt.msg.v.val_2b))
+    && (forall pkt | pkt in ts.t_replicas[1].v.replica.proposer.received_1b_packets && pkt.msg.RslMessage_1b? :: forall op | op in pkt.msg.votes :: RequestBatchSrcInClientIds(ts, pkt.msg.votes[op].max_val))
 
-    && (forall idx | 0 <= idx < |s.t_replicas|
+    && (forall idx | 0 <= idx < |ts.t_replicas|
         ::
-        && (var uls := s.t_replicas[idx].v.replica.learner.unexecuted_learner_state;
-            forall opn | opn in uls :: RequestBatchSrcInClientIds(s, uls[opn].candidate_learned_value)
+        && (var uls := ts.t_replicas[idx].v.replica.learner.unexecuted_learner_state;
+            forall opn | opn in uls :: RequestBatchSrcInClientIds(ts, uls[opn].candidate_learned_value)
             )
-        && (s.t_replicas[idx].v.replica.executor.next_op_to_execute.OutstandingOpKnown?
-            ==> RequestBatchSrcInClientIds(s, s.t_replicas[idx].v.replica.executor.next_op_to_execute.v)
+        && (ts.t_replicas[idx].v.replica.executor.next_op_to_execute.OutstandingOpKnown?
+            ==> RequestBatchSrcInClientIds(ts, ts.t_replicas[idx].v.replica.executor.next_op_to_execute.v)
     )
     )
 }
 
 
 
-predicate PacketsBallotInvariant(s:TimestampedRslState) {
-    forall pkt | pkt in s.undeliveredPackets :: ExistingPacketsBallot(pkt)
+predicate PacketsBallotInvariant(ts:TimestampedRslState) {
+    forall pkt | pkt in ts.undeliveredPackets :: ExistingPacketsBallot(pkt)
 }
 
 predicate ExistingPacketsBallot(pkt:TimestampedLPacket<EndPoint, RslMessage>) {
@@ -272,16 +273,17 @@ predicate ExistingPacketsBallot(pkt:TimestampedLPacket<EndPoint, RslMessage>) {
 }
 
 // Things that are true before 2a packets are sent out by the leader
-predicate Before_2a_Sent_Invariant(s:TimestampedRslState, opn:OperationNumber) 
-    requires |s.t_replicas| > 2
+predicate Before_2a_Sent_Invariant(ts:TimestampedRslState, opn:OperationNumber) 
+    requires |ts.t_replicas| > 2
 {
-    var l := s.t_replicas[1];
+    var l := ts.t_replicas[1];
     var r := l.v.replica;
-    && (!exists pkt :: pkt in s.t_environment.sentPackets && IsNew2aPacket(pkt, opn))
+    && (!exists pkt :: pkt in ts.t_environment.sentPackets && IsNew2aPacket(pkt, opn))
+    && (!exists pkt :: pkt in ts.t_environment.sentPackets && IsNew2bPacket(pkt, opn))
     && TimeLe(l.ts, NewLeaderInitTS)     // leader timestamp
     && l.v.nextActionIndex == 3          // leader action index is 3
-    && LeaderSet1bContainsRequest(s)
-    && s.t_replicas[1].v.nextActionIndex == 3
+    && LeaderSet1bContainsRequest(ts)
+    && ts.t_replicas[1].v.nextActionIndex == 3
     && r.proposer.current_state == 2
     && r.proposer.election_state.current_view == Ballot(1, 1)
     && r.proposer.max_ballot_i_sent_1a == Ballot(1, 1)
@@ -289,13 +291,25 @@ predicate Before_2a_Sent_Invariant(s:TimestampedRslState, opn:OperationNumber)
 }
 
 // Things that are true after 2a packets are sent out by the leader
-predicate After_2a_Sent_Invariant(s:TimestampedRslState, opn:OperationNumber) 
-    requires |s.t_replicas| > 2
+predicate Before_2b_Sent_Invariant(ts:TimestampedRslState, opn:OperationNumber) 
+    requires |ts.t_replicas| > 2
 {
-    var l := s.t_replicas[1];
+    var l := ts.t_replicas[1];
     var r := l.v.replica;
-    && (exists pkt :: pkt in s.t_environment.sentPackets && IsNew2aPacket(pkt, opn))
-    && PerformanceGuarantee_2a(s, opn)
+    && (exists pkt :: pkt in ts.t_environment.sentPackets && IsNew2aPacket(pkt, opn))
+    && (!exists pkt :: pkt in ts.t_environment.sentPackets && IsNew2bPacket(pkt, opn))
+    && PerformanceGuarantee_2a(ts, opn)
+    && r.proposer.current_state == 2
+    && r.proposer.next_operation_number_to_propose > opn
+}
+
+predicate After_2b_Sent_Invariant(ts:TimestampedRslState, opn:OperationNumber) 
+    requires |ts.t_replicas| > 2
+{
+    var l := ts.t_replicas[1];
+    var r := l.v.replica;
+    && exists pkt :: pkt in ts.t_environment.sentPackets && IsNew2bPacket(pkt, opn)
+    && PerformanceGuarantee_2a(ts, opn)
     && r.proposer.current_state == 2
     && r.proposer.next_operation_number_to_propose > opn
 }
@@ -311,6 +325,12 @@ predicate IsNew2aPacket(pkt:TimestampedRslPacket, opn:OperationNumber) {
     && pkt.msg.v.RslMessage_2a?
     && pkt.msg.v.bal_2a == Ballot(1, 1)
     && pkt.msg.v.opn_2a == opn
+}
+
+predicate IsNew2bPacket(pkt:TimestampedRslPacket, opn:OperationNumber) {
+    && pkt.msg.v.RslMessage_2b?
+    && pkt.msg.v.bal_2b == Ballot(1, 1)
+    && pkt.msg.v.opn_2b == opn
 }
 
 }
