ironfleet/src/Dafny/Distributed/Protocol/RSL/FailureProof/Phase2Proof_toplevel.i.dfy
@@ -6,7 +6,7 @@ import opened RslPhase2Proof_postFail_i
 import opened Rs2Phase2Proof_Helper
 
 
-
+/* Main Invariant */
 lemma PerfInvariantMaintained(s:TimestampedRslState, s':TimestampedRslState, req_time:Timestamp, opn:OperationNumber)
     requires RslAssumption(s) && RslAssumption(s')
     requires RslConsistency(s) && RslConsistency(s')
@@ -17,8 +17,14 @@ lemma PerfInvariantMaintained(s:TimestampedRslState, s':TimestampedRslState, req
     PacketsBallotInvariant_Maintained(s, s', opn);
     AlwaysInvariant_Maintained(s, s', opn);
     
-    if !exists pkt :: pkt in s.t_environment.sentPackets && IsNew2aPacket(pkt, opn) {
-        Before2a_to_BeforeOrAfter2a(s, s', opn);
+    if (!exists pkt :: pkt in s.t_environment.sentPackets && IsNew2aPacket(pkt, opn))
+    && (!exists pkt :: pkt in s.t_environment.sentPackets && IsNew2bPacket(pkt, opn)) 
+    {
+        Before2a_to_MaybeBefore2b(s, s', opn);
+    } else if (exists pkt :: pkt in s.t_environment.sentPackets && IsNew2aPacket(pkt, opn))
+        && (!exists pkt :: pkt in s.t_environment.sentPackets && IsNew2bPacket(pkt, opn))  
+    {
+        Before2b_to_MaybeAfter2b(s, s', opn);
     }
 
     assert AlwaysInvariant(s');        
@@ -34,6 +40,7 @@ lemma PerfInvariantMaintained(s:TimestampedRslState, s':TimestampedRslState, req
 *                                         Lemmas                                         *
 *****************************************************************************************/
 
+/* Proof that PacketsBallotInvariant is maintained */
 lemma PacketsBallotInvariant_Maintained(ts:TimestampedRslState, ts':TimestampedRslState, opn:OperationNumber) 
     requires RslAssumption(ts) && RslAssumption(ts')
     requires RslConsistency(ts') && RslConsistency(ts')
@@ -55,14 +62,16 @@ lemma PacketsBallotInvariant_Maintained(ts:TimestampedRslState, ts':TimestampedR
 }
 
 
-lemma Before2a_to_BeforeOrAfter2a(ts:TimestampedRslState, ts':TimestampedRslState, opn:OperationNumber) 
+/* Proof that a Before_2a_Sent state transitions to a Before_2a_Sent state or 
+* Before_2b_Sent state */
+lemma Before2a_to_MaybeBefore2b(ts:TimestampedRslState, ts':TimestampedRslState, opn:OperationNumber) 
     requires RslAssumption(ts) && RslConsistency(ts)
     requires RslAssumption(ts') && RslConsistency(ts')
     requires PacketsBallotInvariant(ts) && PacketsBallotInvariant(ts')
     requires TimestampedRslNext(ts, ts')
     requires RslPerfInvariant(ts, opn)
     requires Before_2a_Sent_Invariant(ts, opn);
-    ensures Before_2a_Sent_Invariant(ts', opn) || After_2a_Sent_Invariant(ts', opn);
+    ensures Before_2a_Sent_Invariant(ts', opn) || Before_2b_Sent_Invariant(ts', opn);
 {
     if TimestampedRslNextEnvironment(ts, ts') {
         assert Before_2a_Sent_Invariant(ts', opn);
@@ -71,10 +80,26 @@ lemma Before2a_to_BeforeOrAfter2a(ts:TimestampedRslState, ts':TimestampedRslStat
     var idx, tios:seq<TimestampedLIoOp<NodeIdentity, RslMessage>> :| TimestampedRslNextOneReplica(ts, ts', idx, tios);
     var nextActionIndex := ts.t_replicas[idx].v.nextActionIndex;
     if idx != 1 {
-        assert Before_2a_Sent_Invariant(ts', opn);
+        Before2a_to_Before2a_NonLeaderAction(ts, ts', opn, idx, tios);
         return;
     }
-    Before2a_to_After2a(ts, ts', opn, tios);
+    Before2a_to_Before2b(ts, ts', opn, tios);
 }
 
+
+/* Proof that a Before_2b_Sent state transitions to a Before_2b_Sent state or 
+* After_2b_Sent state */
+lemma Before2b_to_MaybeAfter2b(ts:TimestampedRslState, ts':TimestampedRslState, opn:OperationNumber) 
+    requires RslAssumption(ts) && RslConsistency(ts)
+    requires RslAssumption(ts') && RslConsistency(ts')
+    requires PacketsBallotInvariant(ts) && PacketsBallotInvariant(ts')
+    requires TimestampedRslNext(ts, ts')
+    requires RslPerfInvariant(ts, opn)
+    requires Before_2b_Sent_Invariant(ts, opn);
+    ensures Before_2b_Sent_Invariant(ts', opn) || After_2b_Sent_Invariant(ts', opn);
+{
+    // TODO
+    assume false;
+    assert Before_2b_Sent_Invariant(ts', opn) || After_2b_Sent_Invariant(ts', opn);
+}
 }
