ironfleet/src/Dafny/Distributed/Protocol/RSL/FailureProof/verify.sh
@@ -1,7 +1,12 @@
 #!/bin/bash -li
 
+echo "Verifying (long) Phase2Proof_helper.i.dfy"
 dafnylong Phase2Proof_helper.i.dfy | grep -iv "Warning"
 
+echo ""
+echo "Verifying Phase2Proof.i.dfy"
 dafny Phase2Proof.i.dfy | grep -iv "Warning"
 
+echo ""
+echo "Verifying Phase2Proof_toplevel.i.dfy"
 dafny Phase2Proof_toplevel.i.dfy | grep -iv "Warning"
